Moved a bunch of stuff from concurrency/juicy/semax_invariant to concurrency/juicy/Clight_mem_ok, that relates to well-formedness properties useful _not only_ in the CSL progress and preservation proofs, but also in the Clight_new_Clight_safety proof.  Sometime soon, mem_wd2 (both the predicate and the entire file) should be removed.

concurrency/juicy/Clight_mem_ok.v
@@ -4,6 +4,7 @@ Require Import compcert.lib.Maps.
 Require Import compcert.common.Values.
 Require Import compcert.common.Globalenvs.
 Require Import compcert.common.Memory.
+Require Import VST.concurrency.common.permissions.
 Require Import compcert.cfrontend.Ctypes.
 Require Import compcert.cfrontend.Clight.
 Require Import VST.sepcomp.event_semantics.
@@ -13,121 +14,288 @@ Require Import VST.msl.eq_dec.
 Require Import BinNums.
 Require Import List. Import ListNotations.
 Require Import VST.msl.Coqlib2.
-
+Require VST.concurrency.compiler.mem_equiv.
+Require Import VST.concurrency.common.threadPool.
 Set Bullet Behavior "Strict Subproofs".
+Import Memory.
+Import ThreadPool.
 
+Arguments sizeof {env} t.
 
 Section GE.
+
 Variable ge: Clight.genv.
+
+Definition maxedmem (m: mem) :=
+  restrPermMap (mem_max_lt_max m).
+
+Definition mem_wellformed (m: mem) :=
+ Mem.inject_neutral (Mem.nextblock m) (maxedmem m) /\
+  Ple (Genv.genv_next ge) (Mem.nextblock m).
+
+Lemma access_at_restr_Cur: 
+ forall loc p m Hlt, access_at (@restrPermMap p m Hlt) loc Cur =  p !! (fst loc) (snd loc).
+Proof.
+intros.
+destruct loc.
+rewrite <- restrPermMap_Cur with (m:=m) (Hlt:=Hlt).
+reflexivity.
+Qed.
+
+Lemma access_at_restr_Max: 
+ forall loc p m Hlt, access_at (@restrPermMap p m Hlt) loc Max =  access_at m loc Max.
+Proof.
+intros.
+destruct loc.
+simpl.
+change (permission_at (restrPermMap Hlt) b z Max = permission_at m b z Max).
+rewrite restrPermMap_Max.
+unfold getMaxPerm.
+rewrite PMap.gmap.
+reflexivity.
+Qed.
+
+Lemma access_at_maxedmem: 
+ forall k m loc, access_at (maxedmem m) loc k =  access_at m loc Max.
+Proof.
+intros.
+destruct loc.
+unfold maxedmem.
+destruct k.
+apply access_at_restr_Max.
+rewrite access_at_restr_Cur.
+unfold getMaxPerm.
+rewrite PMap.gmap.
+reflexivity.
+Qed.
+
+Lemma maxedmem_neutral:
+  forall m,
+ Mem.inject_neutral (Mem.nextblock (maxedmem m)) (maxedmem m) ->
+  Mem.inject_neutral (Mem.nextblock m) m.
+Proof.
+intros.
+unfold Mem.inject_neutral in *.
+inv H.
+constructor; intros; simpl in *.
+-
+unfold Mem.flat_inj in H.
+if_tac in H; inv H.
+rewrite Z.add_0_r. auto.
+-
+eapply mi_align; eauto.
+intros ? ?.
+unfold maxedmem.
+rewrite mem_equiv.restr_Max_equiv. eauto.
+-
+apply mi_memval; auto.
+clear - H0.
+rewrite perm_access in H0.
+rewrite perm_access.
+eapply perm_order''_trans; try eassumption.
+clear H0.
+rewrite access_at_maxedmem.
+apply access_cur_max.
+Qed.
+
+Lemma mem_equiv_restr_max:
+ forall m j (k: permMapLt j (getMaxPerm m)),
+mem_equiv.mem_equiv (restrPermMap (mem_max_lt_max (@restrPermMap j m k)))
+  (restrPermMap (mem_max_lt_max m)).
+Proof.
+intros.
+constructor.
+-
+red.
+etransitivity.
+apply mem_equiv.getCur_restr.
+fold (maxedmem m).
+intro b.
+extensionality z.
+rewrite getCurPerm_correct.
+rewrite getMaxPerm_correct.
+unfold permission_at.
+symmetry.
+pose proof (access_at_maxedmem Cur m (b,z)).
+unfold access_at in H.
+simpl fst in H; simpl snd in H.
+rewrite H.
+symmetry.
+pose proof (restrPermMap_Max k b z).
+unfold permission_at in H0.
+rewrite getMaxPerm_correct in H0.
+apply H0.
+-
+rewrite !mem_equiv.restr_Max_equiv.
+reflexivity.
+-
+rewrite !mem_equiv.restr_content_equiv.
+reflexivity.
+-
+reflexivity.
+Qed.
+
 
 Section CTL_OK.
   Variable nextb : block.
+Definition val_wellformed (v: val) : Prop :=
+   Val.inject (Mem.flat_inj nextb) v v.
 
-Definition block_ok (b: block) := Plt b nextb.
+Definition block_wellformed (b: block) := Plt b nextb.
 
-Definition val_ok (v: val) : Prop := 
- match v with
- | Vptr b _ => block_ok b
- | _ => True
- end.
+Definition venv_wellformed (ve: Clight.env) :=
+  forall i bt, PTree.get i ve = Some bt -> block_wellformed (fst bt).
 
-Definition venv_ok (ve: Clight.env) :=
-  forall i bt, PTree.get i ve = Some bt -> block_ok (fst bt).
+Definition tenv_wellformed (te: Clight.temp_env) :=
+  forall i (v: val), PTree.get i te = Some v -> val_wellformed v.
 
-Definition tenv_ok (te: Clight.temp_env) :=
-  forall i (v: val), PTree.get i te = Some v -> val_ok v.
-
-Fixpoint cont_ok (k: cont) := 
+Fixpoint cont_wellformed (k: cont) := 
  match k with
  | Kstop _ => True
- | Kseq _ k' => cont_ok k'
- | Kloop1 _ _ k' => cont_ok k'
- | Kloop2 _ _ k' => cont_ok k'
- | Kswitch k' => cont_ok k'
- | Kcall _ _ ve te k' => venv_ok ve /\ tenv_ok te /\ cont_ok k'
+ | Kseq _ k' => cont_wellformed k'
+ | Kloop1 _ _ k' => cont_wellformed k'
+ | Kloop2 _ _ k' => cont_wellformed k'
+ | Kswitch k' => cont_wellformed k'
+ | Kcall _ _ ve te k' => venv_wellformed ve /\ tenv_wellformed te /\ cont_wellformed k'
  end.
 
-Definition corestate_ok (q: Clight_core.state) : Prop :=
+Definition core_wellformed (q: Clight_core.state) : Prop :=
  match q with
- | Clight_core.State _ _ k ve te => venv_ok ve /\ tenv_ok te /\ cont_ok k
+ | Clight_core.State _ _ k ve te => venv_wellformed ve /\ tenv_wellformed te /\ cont_wellformed k
  | Clight_core.Callstate f args k =>
-       Forall val_ok args /\  cont_ok k
- | Clight_core.Returnstate v k => val_ok v /\ cont_ok k
+       Forall val_wellformed args /\  cont_wellformed k
+ | Clight_core.Returnstate v k => val_wellformed v /\ cont_wellformed k
  end.
 
 End CTL_OK.
 
+Definition ctl_wellformed {res : semantics.Resources} {sem: semantics.Semantics}
+   (core_wellformed: block -> semantics.semC -> Prop)
+    m ctl :=
+ match ctl with
+    | Krun q => core_wellformed (Mem.nextblock m) q
+    | Kblocked q => core_wellformed (Mem.nextblock m) q
+                              /\ semantics.at_external (semantics.csem (msem (@semantics.semSem sem))) q m <> None
+    | Kresume q v => core_wellformed (Mem.nextblock m) q /\ semantics.at_external (semantics.csem (msem (@semantics.semSem sem))) q m <> None /\ v = Vundef
+    | Kinit v1 v2 => val_wellformed (Mem.nextblock m) v1 /\ val_wellformed (Mem.nextblock m) v2
+    end.
 
+Definition threads_wellformed
+   {res : semantics.Resources} {sem: semantics.Semantics}
+   {core_wellformed: block -> semantics.semC -> Prop}
+   m tp  :=
+  forall i (cnti : @containsThread res sem OrdinalPool.OrdinalThreadPool tp i),
+     ctl_wellformed core_wellformed m (getThreadC cnti).
+
+End GE.
+
+Module Test.
+Require Import VST.concurrency.juicy.JuicyMachineModule.
+Definition juicy_threads_wellformed ge m tp :=
+   @threads_wellformed _ (@THE_JUICY_MACHINE.JSem ge) core_wellformed m tp.
+
+Definition dry_threads_wellformed ge m tp :=
+   @threads_wellformed _ (@ClightSemanticsForMachines.Clight_newSem ge) core_wellformed m tp.
+End Test.
+
+Lemma cl_step_wellformed:
+  forall ge m c pm Hlt c' m',
+      mem_wellformed ge m ->
+      core_wellformed (Mem.nextblock m) c ->
+      Clight_core.cl_step ge c (@restrPermMap pm m Hlt) c' m' ->
+      mem_wellformed ge m' /\ 
+      core_wellformed (Mem.nextblock m') c'.
+Admitted.  (* Santiago will prove this, generically over all injections not just flat ones *)
+
+Lemma initial_core_wellformed:
+  forall ge v args c m,
+     Clight_core.cl_initial_core ge v args c ->
+     Clight_core.arg_well_formed args m ->
+     Smallstep.globals_not_fresh ge m ->
+     core_wellformed (Mem.nextblock m) c.
+Admitted.
 
 Section ALLOC_OK.
 Variable nextb: positive.
 Variable nextb': positive.
 Variable LESS:  (nextb <= nextb')%positive.
 
-Lemma alloc_block_ok: forall b, block_ok nextb b -> block_ok nextb' b.
+Lemma alloc_block_wellformed: forall b, block_wellformed nextb b -> block_wellformed nextb' b.
 Proof.
 intros.
 red in H|-*. eapply Pos.lt_le_trans; eauto.
 Qed.
 
-Lemma alloc_val_ok: forall v, val_ok nextb v -> val_ok nextb' v.
+Lemma alloc_val_wellformed: forall v, val_wellformed nextb v -> val_wellformed nextb' v.
 Proof.
-intros; destruct v; auto.
-red in H|-*. eapply alloc_block_ok; eauto.
+intros; destruct v; try solve [constructor].
+hnf in H|-*.
+inv H; apply Val.inject_ptr with delta; auto.
+unfold Mem.flat_inj in *.
+destruct (plt b nextb); inv H3.
+rewrite if_true; auto.
+eapply Plt_Ple_trans; eauto.
 Qed.
 
-Lemma alloc_venv_ok: forall ve, venv_ok nextb ve -> venv_ok nextb' ve.
-Proof.
-intros.
-red in H|-*; intros.
-eapply alloc_block_ok; eauto.
-Qed.
-
-Lemma alloc_tenv_ok: forall te, tenv_ok nextb te -> tenv_ok nextb' te.
+Lemma alloc_venv_wellformed: forall ve, venv_wellformed nextb ve -> venv_wellformed nextb' ve.
 Proof.
 intros.
 red in H|-*; intros.
-eapply alloc_val_ok; eauto.
+eapply alloc_block_wellformed; eauto.
 Qed.
 
-(*
-Lemma alloc_cont'_ok: forall k, cont'_ok nextb k -> cont'_ok nextb' k.
+Lemma alloc_tenv_wellformed: forall te, tenv_wellformed nextb te -> tenv_wellformed nextb' te.
 Proof.
-destruct k; simpl; auto.
-intros [? ?]; split.
-eapply alloc_venv_ok; eauto.
-eapply alloc_tenv_ok; eauto.
+intros.
+red in H|-*; intros.
+eapply alloc_val_wellformed; eauto.
 Qed.
-*)
 
-Lemma alloc_cont_ok: forall k, cont_ok nextb k -> cont_ok nextb' k.
+Lemma alloc_cont_wellformed: forall k, cont_wellformed nextb k -> cont_wellformed nextb' k.
 Proof.
 induction k; simpl; intros; auto.
 destruct H as [? [? ?]]. split3; auto.
-eapply alloc_venv_ok; eauto.
-eapply alloc_tenv_ok; eauto.
+eapply alloc_venv_wellformed; eauto.
+eapply alloc_tenv_wellformed; eauto.
 Qed.
 
-Lemma alloc_corestate_ok: forall q, corestate_ok nextb q -> corestate_ok nextb' q.
+Lemma alloc_core_wellformed: forall q, 
+    core_wellformed nextb q -> core_wellformed nextb' q.
 Proof.
 destruct q; simpl.
 intros [? [? ?]]; split; [|split].
-eapply alloc_venv_ok; eauto.
-eapply alloc_tenv_ok; eauto.
-eapply alloc_cont_ok; eauto.
+eapply alloc_venv_wellformed; eauto.
+eapply alloc_tenv_wellformed; eauto.
+eapply alloc_cont_wellformed; eauto.
 intros [? ?]; split.
-eapply Forall_impl; try eassumption. apply alloc_val_ok.
-apply alloc_cont_ok; auto.
+eapply Forall_impl; try eassumption. apply alloc_val_wellformed.
+apply alloc_cont_wellformed; auto.
 intros [? ?]; split.
-eapply alloc_val_ok; eauto.
-apply alloc_cont_ok; auto.
+eapply alloc_val_wellformed; eauto.
+apply alloc_cont_wellformed; auto.
 Qed.
 
 End ALLOC_OK.
 
-Lemma set_tenv_ok:
-  forall nextb i (v: val) te, val_ok nextb v -> tenv_ok nextb te ->
-            tenv_ok nextb (PTree.set i v te).
+Lemma alloc_ctl_wellformed: forall {res : semantics.Resources} {sem: semantics.Semantics}
+    (cwf: block -> semantics.semC -> Prop)
+   (H: forall (b b': block) (L: (b <= b')%positive) q, cwf b q -> cwf b' q)
+   (Hat: forall s m m', 
+   semantics.at_external (semantics.csem semantics.semSem) s m =
+   semantics.at_external (semantics.csem semantics.semSem) s m')
+    m m' c, 
+    Ple (Mem.nextblock m) (Mem.nextblock m') ->
+    ctl_wellformed cwf m c -> ctl_wellformed cwf m' c.
+Proof.
+intros.
+destruct c; simpl in *; decompose [and] H1; repeat split; eauto;
+try eapply alloc_val_wellformed; eauto;
+erewrite <- Hat; eauto.
+Qed.
+
+Lemma set_tenv_wellformed:
+  forall nextb i (v: val) te, val_wellformed nextb v -> tenv_wellformed nextb te ->
+            tenv_wellformed nextb (PTree.set i v te).
 Proof.
 intros.
 hnf in H0|-*.
@@ -138,9 +306,9 @@ rewrite PTree.gso in H1 by auto.
 apply H0 in H1. auto.
 Qed.
 
-Lemma set_venv_ok:
-  forall nextb i v ve, block_ok nextb (fst v) -> venv_ok nextb ve ->
-            venv_ok nextb (PTree.set i v ve).
+Lemma set_venv_wellformed:
+  forall nextb i v ve, block_wellformed nextb (fst v) -> venv_wellformed nextb ve ->
+            venv_wellformed nextb (PTree.set i v ve).
 Proof.
 intros.
 hnf in H0|-*.
@@ -151,71 +319,79 @@ rewrite PTree.gso in H1 by auto.
 apply H0 in H1. auto.
 Qed.
 
-Lemma sem_add_ptr_int_ok:
-  forall nextb ty si v1 v2 v,
-  val_ok nextb v1 ->
-  val_ok nextb v2 ->
+Lemma sem_add_ptr_int_wellformed:
+  forall ge nextb ty si v1 v2 v,
+  val_wellformed nextb v1 ->
+  val_wellformed nextb v2 ->
   Cop.sem_add_ptr_int (genv_cenv ge) ty si v1 v2 = Some v -> 
-  val_ok nextb v.
+  val_wellformed nextb v.
 Proof.
 intros.
 unfold Cop.sem_add_ptr_int in H1.
 destruct v1; try discriminate;
 destruct v2; try discriminate.
-destruct Archi.ptr64; inv H1.  auto. 
-inv H1; auto.
+destruct Archi.ptr64; inv H1.
+constructor.
+inv H1.
+inv H.
+apply Val.inject_ptr with delta; auto.
+apply mem_lemmas.flatinj_E in H4. destruct H4 as [? [? ?]]; subst.
+rewrite Ptrofs.add_zero. auto.
 Qed.
 
-Lemma sem_add_ptr_long_ok:
-  forall nextb ty v1 v2 v,
-  val_ok nextb v1 ->
-  val_ok nextb v2 ->
+Lemma sem_add_ptr_long_wellformed:
+  forall ge nextb ty v1 v2 v,
+  val_wellformed nextb v1 ->
+  val_wellformed nextb v2 ->
   Cop.sem_add_ptr_long (genv_cenv ge) ty v1 v2 = Some v -> 
-  val_ok nextb v.
+  val_wellformed nextb v.
 Proof.
 intros.
 unfold Cop.sem_add_ptr_long in H1.
 destruct v1; try discriminate;
 destruct v2; try discriminate.
-destruct Archi.ptr64; inv H1.  auto. 
-inv H1; auto.
+destruct Archi.ptr64; inv H1. constructor.
+inv H1.
+inv H.
+apply Val.inject_ptr with delta; auto.
+apply mem_lemmas.flatinj_E in H4. destruct H4 as [? [? ?]]; subst.
+rewrite Ptrofs.add_zero. auto.
 Qed.
 
-Lemma sem_cast_ok:
+Lemma sem_cast_wellformed:
   forall nextb v1 t1 t2 m v,
-    val_ok nextb v1 ->
+    val_wellformed nextb v1 ->
     Cop.sem_cast v1 t1 t2 m = Some v ->
-     val_ok nextb v.
+     val_wellformed nextb v.
 Proof.
 intros.
 unfold Cop.sem_cast in H0.
 destruct (Cop.classify_cast t1 t2); try discriminate;
 destruct v1; try discriminate;
-try solve [inv H0; auto].
-destruct (Cop.cast_float_int si2 f); inv H0; auto.
-destruct (Cop.cast_single_int si2 f); inv H0; auto.
-destruct (Cop.cast_float_long si2 f); inv H0; auto.
-destruct (Cop.cast_single_long si2 f); inv H0; auto.
-destruct Archi.ptr64; inv H0; auto.
-destruct (Mem.weak_valid_pointer m b (Ptrofs.unsigned i)); inv H2; auto.
-hnf; auto.
+try solve [inv H0; auto; constructor].
+destruct (Cop.cast_float_int si2 f); inv H0; try constructor.
+destruct (Cop.cast_single_int si2 f); inv H0; try constructor.
+destruct (Cop.cast_float_long si2 f); inv H0; try constructor.
+destruct (Cop.cast_single_long si2 f); inv H0; try constructor.
+destruct Archi.ptr64; inv H0; auto; try constructor.
+destruct (Mem.weak_valid_pointer m b (Ptrofs.unsigned i)); inv H2; try constructor.
 if_tac in H0; inv H0; auto.
 if_tac in H0; inv H0; auto.
 Qed.
 
-Lemma val_of_bool_ok:
-  forall nextb b, val_ok nextb (Val.of_bool b).
+Lemma val_of_bool_wellformed:
+  forall nextb b, val_wellformed nextb (Val.of_bool b).
 Proof.
-intros. destruct b; hnf; auto.
+intros. destruct b; hnf; constructor.
 Qed.
 
-Lemma sem_cmp_ok: 
+Lemma sem_cmp_wellformed: 
   forall nextb op v1 t1 v2 t2 m v,
  Cop.sem_cmp op v1 t1 v2 t2 m = Some v ->
- val_ok nextb v1 -> val_ok nextb v2 -> val_ok nextb v.
+ val_wellformed nextb v1 -> val_wellformed nextb v2 -> val_wellformed nextb v.
 Proof.
 intros.
-pose proof (val_of_bool_ok nextb).
+pose proof (val_of_bool_wellformed nextb).
 unfold Cop.sem_cmp in H.
 destruct (Cop.classify_cmp t1 t2); try discriminate.
 unfold Cop.cmp_ptr in H.
@@ -243,8 +419,8 @@ destruct (Cop.sem_cast v1 t1
         (Cop.binarith_type (Cop.classify_binarith t1 t2)) m) eqn:?; try discriminate.
 destruct (Cop.sem_cast v2 t2
         (Cop.binarith_type (Cop.classify_binarith t1 t2)) m) eqn:?; try discriminate.
-eapply sem_cast_ok in Heqo; eauto.
-eapply sem_cast_ok in Heqo0; eauto.
+eapply sem_cast_wellformed in Heqo; eauto.
+eapply sem_cast_wellformed in Heqo0; eauto.
 destruct (Cop.classify_binarith t1 t2); try discriminate.
 destruct v0;  try discriminate.
 destruct v3;  try discriminate.
@@ -260,17 +436,17 @@ destruct v3;  try discriminate.
 inv H; auto.
 Qed.
 
-Lemma binary_operation_ok:
-forall nextb (op : Cop.binary_operation) (v1 : val) (t1 : type) 
+Lemma binary_operation_wellformed:
+forall ge nextb (op : Cop.binary_operation) (v1 : val) (t1 : type) 
   (v2 : val) (t2 : type) (m : mem) (v : val),
-  val_ok nextb v1 ->
-  val_ok nextb v2 ->
+  val_wellformed nextb v1 ->
+  val_wellformed nextb v2 ->
   Cop.sem_binary_operation (Clight.genv_cenv ge) op v1 t1 v2 t2 m = Some v ->
-  val_ok nextb v.
+  val_wellformed nextb v.
 Proof.
 intros.
  destruct op; simpl in *;
-   try solve [revert H1 H H0; apply sem_cmp_ok];
+   try solve [revert H1 H H0; apply sem_cmp_wellformed];
 try solve [
   match type of H1 with ?A _ _ _ _ _ = _ => unfold A in H1 end;
    unfold Cop.sem_binarith in H1;
@@ -278,77 +454,83 @@ try solve [
          (Cop.binarith_type (Cop.classify_binarith t1 t2)) m) eqn:?; try discriminate;
    destruct (Cop.sem_cast v2 t2
          (Cop.binarith_type (Cop.classify_binarith t1 t2)) m) eqn:?; try discriminate;
-   eapply sem_cast_ok in Heqo; eauto;
-   eapply sem_cast_ok in Heqo0; eauto;
+   eapply sem_cast_wellformed in Heqo; eauto;
+   eapply sem_cast_wellformed in Heqo0; eauto;
    destruct (Cop.classify_binarith t1 t2); try discriminate;
-   try solve [destruct v0; inv H1; destruct v3; inv H3; auto];
+   try solve [destruct v0; inv H1; destruct v3; inv H3; constructor];
    destruct v0; inv H1; destruct v3; inv H3; destruct s; inv H2;
-   revert H3; simple_if_tac; intro H3; inv H3; auto].
+   revert H3; simple_if_tac; intro H3; inv H3; constructor].
 - unfold Cop.sem_add in H1.
    destruct (Cop.classify_add t1 t2);
-   try solve [eapply sem_add_ptr_int_ok; try eapply H1; eauto];
-   try solve [eapply sem_add_ptr_long_ok; try eapply H1; eauto].
+   try solve [eapply sem_add_ptr_int_wellformed; try eapply H1; eauto];
+   try solve [eapply sem_add_ptr_long_wellformed; try eapply H1; eauto].
    unfold Cop.sem_binarith in H1.
    destruct (Cop.sem_cast v1 t1
          (Cop.binarith_type (Cop.classify_binarith t1 t2)) m) eqn:?; try discriminate.
    destruct (Cop.sem_cast v2 t2
          (Cop.binarith_type (Cop.classify_binarith t1 t2)) m) eqn:?; try discriminate.
-   eapply sem_cast_ok in Heqo; eauto.
-   eapply sem_cast_ok in Heqo0; eauto.
+   eapply sem_cast_wellformed in Heqo; eauto.
+   eapply sem_cast_wellformed in Heqo0; eauto.
    destruct (Cop.classify_binarith t1 t2); try discriminate;
-   try solve [destruct v0; inv H1; destruct v3; inv H3; auto].
+   try solve [destruct v0; inv H1; destruct v3; inv H3; constructor].
 - unfold Cop.sem_sub in H1.
    destruct (Cop.classify_sub t1 t2).
-   destruct v1; try discriminate;
-   destruct v2; try discriminate; destruct Archi.ptr64; try discriminate; inv H1; auto.
-   destruct v1; try discriminate;
-   destruct v2; try discriminate; destruct Archi.ptr64; try discriminate; inv H1; auto.
+   destruct v1; try discriminate; 
+   destruct v2; try discriminate; destruct Archi.ptr64; try discriminate; inv H1; auto; try constructor;
+   inv H; econstructor; eauto;
+   apply mem_lemmas.flatinj_E in H4; destruct H4 as [? [? ?]]; subst; rewrite Ptrofs.add_zero; auto.   
+   destruct v1; try discriminate; try constructor;
+   destruct v2; try discriminate; destruct Archi.ptr64; try discriminate; inv H1; auto; try constructor.
    destruct (eq_block b b0); try discriminate.
    destruct (proj_sumbool (zlt 0 (sizeof ty)) &&
        proj_sumbool (zle (sizeof ty) Ptrofs.max_signed)); try discriminate.
    inv H3. unfold Vptrofs. destruct (Archi.ptr64); simpl; auto.
+1,2: inv H; econstructor; eauto;
+   apply mem_lemmas.flatinj_E in H4; destruct H4 as [? [? ?]]; subst; rewrite Ptrofs.add_zero; auto.
    destruct (eq_block b b0); try discriminate.
    destruct (proj_sumbool (zlt 0 (sizeof ty)) &&
        proj_sumbool (zle (sizeof ty) Ptrofs.max_signed)); try discriminate.
-   inv H3. unfold Vptrofs. destruct (Archi.ptr64); simpl; auto.
+   inv H3. unfold Vptrofs. destruct (Archi.ptr64); simpl; auto; constructor.
    destruct v1; try discriminate;
-   destruct v2; try discriminate; destruct Archi.ptr64; try discriminate; inv H1; auto.
+   destruct v2; try discriminate; destruct Archi.ptr64; try discriminate; inv H1; auto; try constructor.
+1,2:   inv H; econstructor; eauto;
+   apply mem_lemmas.flatinj_E in H4; destruct H4 as [? [? ?]]; subst; rewrite Ptrofs.add_zero; auto.
    unfold Cop.sem_binarith in H1.
    destruct (Cop.sem_cast v1 t1
          (Cop.binarith_type (Cop.classify_binarith t1 t2)) m) eqn:?; try discriminate.
    destruct (Cop.sem_cast v2 t2
          (Cop.binarith_type (Cop.classify_binarith t1 t2)) m) eqn:?; try discriminate.
-   eapply sem_cast_ok in Heqo; eauto.
-   eapply sem_cast_ok in Heqo0; eauto.
+   eapply sem_cast_wellformed in Heqo; eauto.
+   eapply sem_cast_wellformed in Heqo0; eauto.
    destruct (Cop.classify_binarith t1 t2); try discriminate;
-   try solve [destruct v0; inv H1; destruct v3; inv H3; auto].
+   try solve [destruct v0; inv H1; destruct v3; inv H3; constructor].
 -
    unfold Cop.sem_shl, Cop.sem_shift in H1.
    destruct (Cop.classify_shift t1 t2); try discriminate;
    destruct v1; try discriminate; destruct v2; try discriminate;
-   revert H1; simple_if_tac; intro H1; inv H1; auto.
+   revert H1; simple_if_tac; intro H1; inv H1; constructor.
 -
    unfold Cop.sem_shr, Cop.sem_shift in H1.
    destruct (Cop.classify_shift t1 t2); try discriminate;
    destruct v1; try discriminate; destruct v2; try discriminate;
-   revert H1; simple_if_tac; intro H1; inv H1; auto.
+   revert H1; simple_if_tac; intro H1; inv H1; constructor.
 Qed.
 
-Lemma loadbytes_proj_ok:
+Lemma loadbytes_proj_wellformed:
   forall m loc ofs sz bl ch q,
-  block_ok (Mem.nextblock m) loc ->
+  block_wellformed (Mem.nextblock m) loc ->
   mem_wd2 m ->
   Mem.loadbytes m loc ofs sz = Some bl ->
-  val_ok (Mem.nextblock m) (Val.load_result ch (proj_value q bl)).
+  val_wellformed (Mem.nextblock m) (Val.load_result ch (proj_value q bl)).
 Proof.
 intros.
-assert (forall ch, val_ok (Mem.nextblock m) (Val.load_result ch Vundef)) 
+assert (forall ch, val_wellformed (Mem.nextblock m) (Val.load_result ch Vundef)) 
  by (intros; destruct ch0; simpl; hnf; auto).
 unfold proj_value.
 destruct bl; auto.
 destruct m0; auto.
 destruct (check_value (size_quantity_nat q) v q (Fragment v q0 n :: bl)) eqn:?H; auto.
-assert (val_ok (Mem.nextblock m) v). {
+assert (val_wellformed (Mem.nextblock m) v). {
  clear - H1 H H0.
  red in H0.
  specialize (H0 loc ofs).
@@ -364,21 +546,20 @@ assert (val_ok (Mem.nextblock m) v). {
  unfold Mem.flat_inj in H6.
  if_tac in H6; inv H6.
  simpl.
- apply H0.
+ econstructor; try eassumption.
+ apply mem_lemmas.flatinj_I; auto.
 }
 unfold Val.load_result.
 destruct ch; try solve [hnf; auto];
 destruct v; try solve [hnf; auto].
-destruct Archi.ptr64; auto.
-hnf; auto.
 Qed.
 
-Lemma deref_loc_ok: 
+Lemma deref_loc_wellformed: 
   forall m loc ofs t1 v,
   mem_wd2 m ->
-  block_ok (Mem.nextblock m) loc ->
+  block_wellformed (Mem.nextblock m) loc ->
   deref_loc t1 m loc ofs v -> 
-  val_ok (Mem.nextblock m) v.
+  val_wellformed (Mem.nextblock m) v.
 Proof.
 intros.
 inv H1; auto.
@@ -391,67 +572,81 @@ destruct (proj_bytes bl) eqn:?H.
 destruct chunk; hnf; auto.
 destruct chunk; try solve [hnf; auto].
 1,2: destruct Archi.ptr64; try solve [hnf; auto].
-all: eapply loadbytes_proj_ok; eauto.
+all: try eapply loadbytes_proj_wellformed in H1; eauto.
+hnf.
+econstructor.
+apply mem_lemmas.flatinj_I; auto.
+rewrite Ptrofs.add_zero; auto.
+econstructor.
+apply mem_lemmas.flatinj_I; auto.
+rewrite Ptrofs.add_zero; auto.
 Qed.
 
-Lemma eval_expr_ok:
-  forall (m : mem) (ve : Clight.env) (te : Clight.temp_env)
+Lemma eval_expr_wellformed:
+  forall ge (m : mem) (ve : Clight.env) (te : Clight.temp_env)
   (a : Clight.expr) (v : val),
 @Smallstep.globals_not_fresh Clight.fundef type (Clight.genv_genv ge) m ->
 mem_wd2 m ->
-venv_ok (Mem.nextblock m) ve ->
-tenv_ok (Mem.nextblock m) te ->
+venv_wellformed (Mem.nextblock m) ve ->
+tenv_wellformed (Mem.nextblock m) te ->
 eval_expr ge ve te m a v -> 
-val_ok (Mem.nextblock m) v
- with eval_lvalue_ok:
-  forall (m : mem) (ve : Clight.env) (te : Clight.temp_env)
+val_wellformed (Mem.nextblock m) v
+ with eval_lvalue_wellformed:
+  forall ge (m : mem) (ve : Clight.env) (te : Clight.temp_env)
   (a : Clight.expr) (v : block) ofs,
 @Smallstep.globals_not_fresh Clight.fundef type (Clight.genv_genv ge) m ->
 mem_wd2 m ->
-venv_ok (Mem.nextblock m) ve ->
-tenv_ok (Mem.nextblock m) te ->
+venv_wellformed (Mem.nextblock m) ve ->
+tenv_wellformed (Mem.nextblock m) te ->
 eval_lvalue ge ve te m a v ofs -> 
-block_ok (Mem.nextblock m) v.
+block_wellformed (Mem.nextblock m) v.
 Proof.
-* clear eval_expr_ok.
+* clear eval_expr_wellformed.
 intros.
-assert (Hof_bool: forall v, val_ok (Mem.nextblock m) (Val.of_bool v))
-    by (intro v'; destruct v'; apply I).
-induction H3; try solve [apply I].
+assert (Hof_bool: forall v, val_wellformed (Mem.nextblock m) (Val.of_bool v))
+       by (intro v'; destruct v'; constructor).
+induction H3; try solve [constructor].
  + apply H2 in H3; auto.
- + apply eval_lvalue_ok in H3; auto.
+ + apply eval_lvalue_wellformed in H3; auto.
+     red in H3.
+     econstructor; eauto. apply mem_lemmas.flatinj_I; auto. rewrite Ptrofs.add_zero; auto.
  + destruct op; simpl in H4. 
      - clear - Hof_bool H4 IHeval_expr.
         unfold Cop.sem_notbool, Cop.bool_val in H4. 
         destruct (Clight.typeof a) as [ | [| | | ] [| ]| | [ | ] |  | | | | ];
-        simpl in H4; try discriminate;
-        try match type of H4 with context [Archi.ptr64] => 
-                          destruct Archi.ptr64; simpl in H4; try discriminate end;
-        try (destruct v1; inv H4; auto;
-           destruct Archi.ptr64; inv H0;
-           destruct (Mem.weak_valid_pointer m b (Ptrofs.unsigned i)); inv H1;
-           apply I).
+        try discriminate;
+        unfold Cop.classify_bool in H4;
+        simpl typeconv in H4; cbv beta zeta iota in H4;
+        try match type of H4 with context [if Archi.ptr64 then Cop.bool_case_l else Cop.bool_case_i]
+            => destruct Archi.ptr64
+        end;
+        destruct v1; inv H4; auto;
+      try match goal with H: option_map _ (if Archi.ptr64 then _ else _) = _ |- _ =>
+        destruct Archi.ptr64; simpl in H; try discriminate end;
+      try match goal with H: option_map _ (if ?A then _ else _) = _ |- _ =>
+        destruct A; inv H; try discriminate end;
+      try apply (Hof_bool false).
     - clear - Hof_bool H4 IHeval_expr.
         unfold Cop.sem_notint, Cop.bool_val in H4. 
         destruct (Clight.typeof a) as [ | [| | | ] [| ]| | [ | ] |  | | | | ];
         simpl in H4; try discriminate;
         try match type of H4 with context [Archi.ptr64] => 
                           destruct Archi.ptr64; simpl in H4; try discriminate end;
-        try (destruct v1; inv H4; auto;
+        try (destruct v1; inv H4; auto; try constructor;
            destruct Archi.ptr64; inv H0;
            destruct (Mem.weak_valid_pointer m b (Ptrofs.unsigned i)); inv H1;
-           apply I).
+           constructor).
     - unfold Cop.sem_neg in H4.
         destruct (Cop.classify_neg (Clight.typeof a)); inv H4;
-        destruct v1; inv H6; auto.
+        destruct v1; inv H6; constructor.
    - unfold Cop.sem_absfloat in H4.
         destruct (Cop.classify_neg (Clight.typeof a)); inv H4;
-        destruct v1; inv H6; auto.
- + eapply binary_operation_ok; try apply H3; eauto.
- + eapply sem_cast_ok; try apply H4; eauto.
- + apply eval_lvalue_ok in H3; auto.
-     eapply deref_loc_ok; try apply H4; auto.
-* clear eval_lvalue_ok.
+        destruct v1; inv H6; constructor.
+ + eapply binary_operation_wellformed; try apply H3; eauto.
+ + eapply sem_cast_wellformed; try apply H4; eauto.
+ + apply eval_lvalue_wellformed in H3; auto.
+     eapply deref_loc_wellformed; try apply H4; auto.
+* clear eval_lvalue_wellformed.
   intros.
   induction H3.
   apply H1 in H3. auto.
@@ -459,41 +654,44 @@ induction H3; try solve [apply I].
   red in H.
   red. apply Genv.genv_symb_range in H4.
   eapply Pos.lt_le_trans; eauto.
-  apply eval_expr_ok in H3; auto.
-  apply eval_expr_ok in H3; auto.
-  apply eval_expr_ok in H3; auto.
+  apply eval_expr_wellformed in H3; auto;
+  inv H3; apply mem_lemmas.flatinj_E in H7; destruct H7 as [? [? ?]]; subst; auto.
+  apply eval_expr_wellformed in H3; auto.
+  inv H3. apply mem_lemmas.flatinj_E in H10; destruct H10 as [? [? ?]]; subst; auto.
+  apply eval_expr_wellformed in H3; auto.
+  inv H3. apply mem_lemmas.flatinj_E in H9; destruct H9 as [? [? ?]]; subst; auto.
 Qed.
 
-Lemma eval_exprlist_ok:
-  forall (m : mem) (ve : Clight.env) (te : Clight.temp_env)
+Lemma eval_exprlist_wellformed:
+  forall ge (m : mem) (ve : Clight.env) (te : Clight.temp_env)
   (al : list Clight.expr) tl (vl : list val),
 @Smallstep.globals_not_fresh Clight.fundef type (Clight.genv_genv ge) m ->
 mem_wd2 m ->
-venv_ok (Mem.nextblock m) ve ->
-tenv_ok (Mem.nextblock m) te ->
+venv_wellformed (Mem.nextblock m) ve ->
+tenv_wellformed (Mem.nextblock m) te ->
 eval_exprlist ge ve te m al tl vl -> 
-Forall (val_ok (Mem.nextblock m)) vl.
+Forall (val_wellformed (Mem.nextblock m)) vl.
 Proof.
 intros.
 induction H3.
 constructor.
-eapply eval_expr_ok in H3; eauto.
+eapply eval_expr_wellformed in H3; eauto.
 constructor; auto.
-eapply sem_cast_ok in H4; eauto.
+eapply sem_cast_wellformed in H4; eauto.
 Qed.
 
-Lemma find_label_ok:
+Lemma find_label_wellformed:
  forall nextb lbl s s' (k : cont) (k' : cont),
-  cont_ok nextb k ->
+  cont_wellformed nextb k ->
   find_label lbl s k = Some (s',k') ->
-  cont_ok nextb k'
-with find_label_ls_ok:
+  cont_wellformed nextb k'
+with find_label_ls_wellformed:
  forall nextb lbl s s' (k : cont) (k' : cont),
-  cont_ok nextb k ->
+  cont_wellformed nextb k ->
   find_label_ls lbl s k = Some (s', k') ->
-  cont_ok nextb k'.
+  cont_wellformed nextb k'.
 Proof.
-* clear find_label_ok.
+* clear find_label_wellformed.
 induction s; simpl; intros; try discriminate.
 -
 destruct (find_label lbl s1
@@ -510,42 +708,42 @@ destruct (find_label lbl s1 (Kloop1 s1 s2 k)) eqn:?; inv H0.
 apply IHs1 in Heqo; auto.
 apply IHs2 in H2; auto.
 -
-eapply find_label_ls_ok in H0; eauto.
+eapply find_label_ls_wellformed in H0; eauto.
 -
 if_tac in H0.
 subst. inv H0. auto.
 apply IHs in H0; auto.
 *
-clear find_label_ls_ok.
+clear find_label_ls_wellformed.
 induction s; intros.
 inv H0.
 simpl in H0.
 destruct (find_label lbl s
          (Kseq (seq_of_labeled_statement s0) k)) eqn:?H; inv H0.
-eapply find_label_ok; try apply H1; eauto.
+eapply find_label_wellformed; try apply H1; eauto.
 repeat constructor; auto.
 apply IHs in H3; auto.
 Qed.
 
-Lemma call_cont_ok_lemma:
+Lemma call_cont_wellformed_lemma:
   forall b k, 
-    cont_ok b k -> cont_ok b (call_cont k).
+    cont_wellformed b k -> cont_wellformed b (call_cont k).
 Proof.
 induction k; simpl; intros; auto.
 Qed.
 
-Lemma mem_ok_goto:
+Lemma mem_wellformed_goto:
  forall f (k k' : cont) (lbl : Clight.label)
        (s' : Clight.statement) (nextb : block),
-  cont_ok nextb k -> 
+  cont_wellformed nextb k -> 
   find_label lbl (fn_body f) (call_cont k) = Some (s', k') ->
-  cont_ok nextb k'.
+  cont_wellformed nextb k'.
 Proof.
 intros.
-apply call_cont_ok_lemma in H.
+apply call_cont_wellformed_lemma in H.
 forget (call_cont k) as k0. clear k; rename k0 into k.
 revert H H0.
-apply find_label_ok.
+apply find_label_wellformed.
 Qed.
 
 Lemma loadbytes_storebytes_wd2:
@@ -621,12 +819,12 @@ inv H1.
 Opaque Mem.free.
 Qed.
 
-Lemma alloc_variables_ok: 
-  forall ve m vl ve' m',
+Lemma alloc_variables_wellformed: 
+  forall ge ve m vl ve' m',
    mem_wd2 m ->
-   venv_ok (Mem.nextblock m) ve ->
+   venv_wellformed (Mem.nextblock m) ve ->
    alloc_variables ge ve m vl ve' m' ->
-   venv_ok (Mem.nextblock m') ve' /\ mem_wd2 m' /\ (Mem.nextblock m <= Mem.nextblock m')%positive.
+   venv_wellformed (Mem.nextblock m') ve' /\ mem_wd2 m' /\ (Mem.nextblock m <= Mem.nextblock m')%positive.
 Proof.
   intros.
   revert ve m H H0 H1; induction vl; simpl; intros.
@@ -639,19 +837,19 @@ Proof.
   apply Mem.nextblock_alloc in H6. rewrite H6.
   apply Ple_succ.
   eapply mem_wd2_alloc; eauto.
-  apply set_venv_ok.
+  apply set_venv_wellformed.
   apply Mem.valid_new_block in H6. red in H6. apply H6.
-  eapply alloc_venv_ok; try eassumption.
+  eapply alloc_venv_wellformed; try eassumption.
   apply Mem.nextblock_alloc in H6. rewrite H6.
   apply Ple_succ.
 Qed.
 
-Lemma bind_parameter_temps_ok:
+Lemma bind_parameter_temps_wellformed:
   forall m fl vl te te',
-    tenv_ok (Mem.nextblock m) te ->
-    Forall (val_ok (Mem.nextblock m))vl ->
+    tenv_wellformed (Mem.nextblock m) te ->
+    Forall (val_wellformed (Mem.nextblock m))vl ->
     bind_parameter_temps fl vl te = Some te' ->
-    tenv_ok (Mem.nextblock m) te'.
+    tenv_wellformed (Mem.nextblock m) te'.
 Proof.
 induction fl; intros; auto.
 inv H1. destruct vl; inv H3. auto.
@@ -660,19 +858,17 @@ destruct a.
 destruct vl; inv H3.
 inv H0.
 apply IHfl in H2; auto.
-apply set_tenv_ok; auto.
+apply set_tenv_wellformed; auto.
 Qed.
-
-End GE.
 
 Lemma inline_external_call_mem_wd:
   forall (ge: genv) ef vargs m vres m',
   Events.external_call ef ge vargs m Events.E0 vres m' ->
   AST.ef_inline ef = true ->
-  Forall (val_ok (Mem.nextblock m)) vargs ->
+  Forall (val_wellformed (Mem.nextblock m)) vargs ->
   Smallstep.globals_not_fresh ge m ->
   mem_wd2 m ->
-  mem_wd2 m' /\ val_ok (Mem.nextblock m') vres /\ (Mem.nextblock m <= Mem.nextblock m')%positive.
+  mem_wd2 m' /\ val_wellformed (Mem.nextblock m') vres /\ (Mem.nextblock m <= Mem.nextblock m')%positive.
 Proof.
 intros.
 destruct ef; try solve [inv H0].
@@ -718,12 +914,15 @@ spec H4. {
  split3; auto.
  clear - H12; admit.
 {
- clear - H5 H6. hnf. destruct vres; auto. red.
+ clear - H5 H6. hnf. destruct vres; auto.
+  apply Val.inject_ptr with 0.
+  apply mem_lemmas.flatinj_I; auto.
   pose proof (Mem.mi_freeblocks _ _ _ H6 b).
   unfold Mem.valid_block in H.
   destruct (plt b (Mem.nextblock m')); auto.
   apply H in n.
   inv H5. congruence.
+  rewrite Ptrofs.add_zero; auto.
 }
  eapply (Events.ec_valid_block EFP) with (b:=Pos.pred (Mem.nextblock m)) in H.
  clear - H.
@@ -740,9 +939,10 @@ inv H4.
 inv H1. inv H8. inv H9.
 split3.
 eapply mem_wd2_store in H5; eauto.
-constructor.
+admit.
 apply Mem.nextblock_store in H5. rewrite H5.
-apply Ple_refl.
+admit.
+admit.
 -
 admit.  (* factor out extcall_properties from the first case above,
    and then use extcall_memcpy_ok *)
@@ -760,13 +960,13 @@ constructor.
 apply Ple_refl.
 Admitted.
 
-Lemma cl_step_ok:
+Lemma cl_step_wellformed':
   forall (ge: genv) c m c' m',
  cl_step ge c m c' m' ->
 Smallstep.globals_not_fresh (Clight.genv_genv ge) m /\
-mem_wd2 m /\ corestate_ok (Mem.nextblock m) c ->
+mem_wd2 m /\ core_wellformed (Mem.nextblock m) c ->
 mem_wd2 m' /\
-corestate_ok (Mem.nextblock m') c' /\
+core_wellformed (Mem.nextblock m') c' /\
 (Mem.nextblock m <= Mem.nextblock m')%positive.
 Proof.
 intros until m'. intro Hstep.
@@ -774,12 +974,13 @@ intros until m'. intro Hstep.
   try (split3; [solve [auto] | solve [auto] | try apply Pos.le_refl]). 
 * (* assign *)
   destruct H5 as [? [? Hk]].
-  eapply eval_expr_ok in H0; eauto.
-  eapply eval_lvalue_ok in H; eauto.
-  eapply sem_cast_ok in H1; eauto.
+  eapply eval_expr_wellformed in H0; eauto.
+  eapply eval_lvalue_wellformed in H; eauto.
+  eapply sem_cast_wellformed in H1; eauto.
   assert (mem_wd.val_valid v m). {
    clear - H1.
     hnf. hnf in H1. destruct v; auto.
+    inv H1. apply mem_lemmas.flatinj_E in H3. apply H3.
  }
   inv H2.
   unfold Mem.storev in H9.
@@ -797,33 +998,33 @@ intros until m'. intro Hstep.
    destruct H2 as [? [? ?]].
    repeat split;  auto.
    2: apply Pos.le_refl.
-   apply set_tenv_ok; auto.
-   eapply eval_expr_ok; eauto.
+   apply set_tenv_wellformed; auto.
+   eapply eval_expr_wellformed; eauto.
 *  destruct H6 as [? [? ?]].
-  eapply eval_expr_ok in H0; try eassumption. (* *)
-  eapply eval_exprlist_ok in H1; eauto.
+  eapply eval_expr_wellformed in H0; try eassumption. (* *)
+  eapply eval_exprlist_wellformed in H1; eauto.
   split3; auto.
   split3; auto.
   apply Pos.le_refl.
 * (* builtin *)
   destruct H4 as [? [? ?]].
-  eapply eval_exprlist_ok in H0; eauto.
+  eapply eval_exprlist_wellformed in H0; eauto.
   exploit inline_external_call_mem_wd; eauto.
   intros [? [? ?]].
   split3; auto. split3; auto.
-  eapply alloc_venv_ok; eauto.
+  eapply alloc_venv_wellformed; eauto.
   destruct optid; auto.
-  apply set_tenv_ok; auto.
-  eapply alloc_tenv_ok; eauto.
-  eapply alloc_tenv_ok; eauto.
-  eapply alloc_cont_ok; eauto.
+  apply set_tenv_wellformed; auto.
+  eapply alloc_tenv_wellformed; eauto.
+  eapply alloc_tenv_wellformed; eauto.
+  eapply alloc_cont_wellformed; eauto.
 * (* return None *)
   rewrite (mem_lemmas.nextblock_freelist _ _ _ H).
   split3.
   eapply mem_wd_freelist; eassumption.
   destruct H2 as [? [? ?]].
   split. hnf; auto.
-  apply call_cont_ok_lemma; auto.
+  apply call_cont_wellformed_lemma; auto.
   apply Pos.le_refl.
 * (* return Some *)
   rewrite (mem_lemmas.nextblock_freelist _ _ _ H1).
@@ -831,48 +1032,49 @@ intros until m'. intro Hstep.
   eapply mem_wd_freelist; eassumption.
   destruct H4 as [? [? ?]]. hnf.
   split.
-  eapply eval_expr_ok in H; eauto.
-  eapply sem_cast_ok; eauto.
-  apply call_cont_ok_lemma; auto.
+  eapply eval_expr_wellformed in H; eauto.
+  eapply sem_cast_wellformed; eauto.
+  apply call_cont_wellformed_lemma; auto.
   apply Pos.le_refl.
 * (* return fall-through *)
   rewrite (mem_lemmas.nextblock_freelist _ _ _ H0).
+   destruct H3 as [? [? ?]].
   split3.
   eapply mem_wd_freelist; eassumption.
-  simpl. destruct H3 as [? [? ?]]. auto.
+  simpl. split; auto. constructor. 
   apply Pos.le_refl.
 * (* goto *)
   split; auto.
   split; [ | apply Pos.le_refl].
   destruct H2 as [? [? ?]]. split; [|split]; auto.
   inv H.
-  eapply mem_ok_goto; eauto.
+  eapply mem_wellformed_goto; eauto.
 * (* call_internal *)
   destruct H2 as [H2' H2].
   inv H.
-  eapply alloc_variables_ok in H6; eauto;
+  eapply alloc_variables_wellformed in H6; eauto;
    [ | clear; hnf; intros; rewrite PTree.gempty in H; inv H].
   destruct H6 as [? [? ?]].
-  eapply bind_parameter_temps_ok in H7; eauto.
+  eapply bind_parameter_temps_wellformed in H7; eauto.
   split3; auto.
   split3; auto.
-  eapply alloc_tenv_ok; eauto.
-  eapply alloc_cont_ok; eauto.
-  eapply alloc_tenv_ok; eauto.
+  eapply alloc_tenv_wellformed; eauto.
+  eapply alloc_cont_wellformed; eauto.
+  eapply alloc_tenv_wellformed; eauto.
   clear. induction (fn_temps f); simpl. intros ? ? ?. rewrite PTree.gempty in H. inv H. destruct a.
-  apply set_tenv_ok; auto. hnf; auto.
+  apply set_tenv_wellformed; auto. hnf; auto.
 * (* call_external inline *)
   destruct H3 as [? ?].
   exploit inline_external_call_mem_wd; eauto.
   intros [? [? ?]]; split3; auto.
   split; auto.
-  eapply alloc_cont_ok; eauto.
+  eapply alloc_cont_wellformed; eauto.
 * (* returnstate *)
   destruct H1.
   split3; auto.
   destruct H2 as [? [? ?]].
   split3; auto.
   destruct optid; auto.
-  apply set_tenv_ok; auto. 
+  apply set_tenv_wellformed; auto. 
   apply Pos.le_refl.
 Qed.
